raft/protocols/Raft/RaftHeader.v
@@ -3,7 +3,12 @@
  * protocol with velisarios.
  !*)
 
-(* find what the quorum file defines, maybe not needed? *)
+(** In general the raft protocol can be seperated into multiple parts:
+ ** Client Interaction
+ ** Leader Election
+ ** Log Replication
+ **)
+
 Require Export Velisarios.Quorum.
 (* the process module provides the abstraction which is implemented by the protocols *)
 Require Export Velisarios.Process.
@@ -12,9 +17,12 @@ Require Export String.
 (*! abstract topology !*)
 (** This section defines the topology of raft which is modeled as an agent
  ** based network. Here a topology describes the set of nodes within the network,
- ** the messages which can be exchanged in the network and the basics context which
- ** can be used by every node, called context. Other basic aspects of the
- ** protocol are also defined here, like progress terms. **)
+ ** the messages which can be exchanged in the network and the basics abstraction context which
+ ** is later filled by the application, because the types are not needed for the protocol.
+ ** Other basic aspects of the protocol are also defined here, like progress terms.
+ **
+ ** Throughout this project types are CamelCase with some obvious exceptions and
+ ** functions are snake_case with some obvious exceptions. **)
 Section RaftHeader.
 
   (* needed? *)
@@ -22,16 +30,16 @@ Section RaftHeader.
   Local Open Scope proc.
 
   (*! Context definition !*)
-  (** The type class raft context provides a set of methods as dependent record.
-   ** The raft context defines some basics which are used throughout all replicas.
-   ** This context shall be binded by some real instance within the rest of the protocol. **)
+  (** The context serves for abstraction of function and entities which types
+   ** are provided by an implementation and can be ignored in the actual protocol. **)
   Class RaftContext :=
     MkRaftContext
       {
-        (* number of faults *)
+        (* number of possible faults *)
         F : nat;
         (* number of replicas needed *)
         num_replicas := (3 * F) + 1;
+
         (* the replicas are only some type *)
         Rep : Set;
         (* replicas have decidable equality *)
@@ -50,29 +58,35 @@ Section RaftHeader.
         clients2nat : Client -> nat_n num_clients;
         (* the projections ist bijective *)
         clients_bij : bijective clients2nat;
-        (* describe the local state machines *)
-        RaftSM_state : Set;
-        (* the initial state of the state machine *)
-        RaftSM_initial_state : RaftSM_state;
         (* this should be the base timerout for the leader election
          * where no followers should start at the same moment with voting. *)
         base_timeout : nat;
         (* the content type for the log *)
-        content_type : Set;
+        Content : Set;
         (* get a textual representation from the content *)
-        content2string : content_type -> string;
+        content2string : Content -> string;
+        (* the result type which gets issued by the internal state update function *)
+        RaftSM_result : Set;
+        (* This is the internal state machine where the
+         * log entries that are committed are processed. *)
+        RaftSM : Set;
+        (* the initial state of the internal state machine *)
+        RaftSM_initial_state : RaftSM;
+        (* the update function for the internal state machine *)
+        RaftSM_update_state : RaftSM -> Content -> RaftSM * RaftSM_result
       }.
+  (** To get this construct clear: The here proposed functions and types are used by the protocol
+   ** but get instantiated in the RaftSim.v file or some other file which uses the raft protocol. **)
 
   (** Declares the context type class as new variable with implicit
-   ** generalization of free terms. Since everything is typed no free terms
-   ** are gneralized? **)
+   ** generalization of free terms. Since everything is typed no free terms are gneralized? **)
   Context { raft_context : RaftContext }.
 
   (*! Nodes !*)
-  (** Define the types of nodes which are used in the system. **)
-  Inductive Raftnode :=
+  (** Nodes are used to distinguish between server's.
+   ** The parameters are defined in the RaftContext and are implemented by the simulation. **)
+  Inductive RaftNode :=
   (* The normal replica node which is either leader or follower.
-   * The parameter is defined in the context as natural number.
    * A replica has three internal states which are hidden by this definition.
    * 1. follower mode: The basic mode where the node is passive and
    *    only responds to incoming messages.
@@ -81,28 +95,27 @@ Section RaftHeader.
    * 3. candidate mode: Used for the leader election and at
    *    this point all nodes are considered as possible candidates.
    * This modes or states are hidden within the replica context. *)
-  | Raftreplica (n : Rep)
-  (* The other node is the client which is in fact outside the agent based system
-   * and only feeds the other nodes with input. The parameter is defined in the context
-   * as natural number *)
-  | Raftclient (n : Client).
+  | replica (n : Rep)
+  (* The other node is the client which is in fact not modeled within COQ.
+   * It is modeled in ocaml outside the protocol and only feeds the input.  *)
+  | client (n : Client).
 
-  (* extract the replica of some node *)
-  Definition node2rep (n : Raftnode) : option Rep :=
+  (** Get the replica parameter of some node. **)
+  Definition replica2rep (n : RaftNode) : option Rep :=
     match n with
-    | Raftreplica n => Some n
+    | replica n => Some n
     | _ => None
     end.
 
-  (* extract the client of some node *)
-  Definition client2rep (n : Raftnode) : option Client :=
+  (** Get the client parameter of some node. **)
+  Definition client2rep (n : RaftNode) : option Client :=
     match n with
-    | Raftclient n => Some n
+    | client n => Some n
     | _ => None
     end.
 
   (** Prove that raft nodes have decidable equality like the one from Leibnitz. **)
-  Lemma RaftnodeDeq : Deq Raftnode.
+  Lemma RaftnodeDeq : Deq RaftNode.
   Proof.
     introv.
     destruct x as [r1|c1], y as [r2|c2].
@@ -114,25 +127,26 @@ Section RaftHeader.
       intro xx. inversion xx. subst. tcsp.
   Defined.
 
-  (** Bind the real node definition as instance to the abstract definition from veliarios. **)
-  Global Instance Raft_I_Node : Node := MkNode Raftnode RaftnodeDeq.
+  (** Bind the real node definition as instance to the abstract definition from velisarios. **)
+  Global Instance Raft_I_Node : Node := MkNode RaftNode RaftnodeDeq.
 
-  (*! TODO: Add more notes to this section!*)
   (*! Quorum instance !*)
-  Lemma Raftreplica_inj : injective Raftreplica.
+  Lemma replica_inj : injective replica.
   Proof.
     introv h; ginv; auto.
   Qed.
 
+  (** Define a quorum as a set of node names with the property of being
+   ** depictable into the set of natural numbers. **)
   Global Instance Raft_I_Quorum : Quorum_context :=
     MkQuorumContext
-      Rep
-      num_replicas
-      rep_deq
-      reps2nat
-      reps_bij
-      Raftreplica
-      Raftreplica_inj.
+      Rep (* the node type *)
+      num_replicas (* size of the set *)
+      rep_deq (* the nodes have to be decidable equality *)
+      reps2nat (* fn which translates nodes to nats *)
+      reps_bij (* node translation is bijective *)
+      replica (* the inductive arm indicates the nodes name *)
+      replica_inj. (* prove that the function is injective *)
 
   (* can we have something like this? *)
   Definition rep2node := Rep -> node_type.
@@ -153,8 +167,7 @@ Section RaftHeader.
   (*Eval simpl in (name_dec (PBFTreplica replica0) (PBFTreplica replica0)).*)
 
   (* We'll return the node as given by our bijection if n < num_nodes,
-     otherwise we return a default value (replica0)
-   *)
+     otherwise we return a default value (replica0) *)
   Definition nat2rep (n : nat) : Rep.
   Proof.
     destruct reps_bij as [f a b].
@@ -169,7 +182,7 @@ Section RaftHeader.
       (seq 0 num_replicas)
       (fun n i => bij_inv reps_bij (mk_nat_n (seq_0_lt i))).
 
-  Definition nreps : list name := map Raftreplica reps.
+  Definition nreps : list name := map replica reps.
 
   Lemma reps_prop : forall (x : Rep), In x reps.
   Proof.
@@ -181,7 +194,7 @@ Section RaftHeader.
       (seq 0 num_clients)
       (fun n i => bij_inv clients_bij (mk_nat_n (seq_0_lt i))).
 
-  Definition nclients : list name := map Raftclient clients.
+  Definition nclients : list name := map client clients.
 
   Lemma clients_prop : forall (x : Client), In x clients.
   Proof.
@@ -210,18 +223,140 @@ Section RaftHeader.
     apply UIP_dec; apply bool_dec.
   Qed.
 
-  (*! Here are the definitions for the types used in within the messages and states !*)
+  (*! Client Interaction !*)
+  (** There are some considerations about how some client interacts with the replicated state
+   ** machine.
+   ** 1. How does the client find the network?
+   ** For simplicity we assume the network has a fixed address and the client knows this address.
+   ** The paper proposes broadcasting or dns lookup for this problem.
+   ** 2. How does a request routes to the leader or the client finds the leader?
+   ** The papers approach is to reject client requests if the server is not the leader and
+   ** the client has to try again. This approach leads to (n+1)/2 attempts to find the current
+   ** leader. The proposed optimization is that the server returns the currently known leader
+   ** to the client.
+   ** The second proposed mechanism is implemented here, where a server forwards the client
+   ** request to the leader. **)
+
+  (*! Linearizable semantics !*)
+  (** To prevent leaders to process a request twice and change the state without
+   ** knowledge for a client RAFT implements a linearizable semantics which has stronger
+   ** guarantees than the at-least-once semantics.
+   ** The idea is that every client registers itself by the network and gets an unique
+   ** session id. Every request from a registered client has a unique serial number.
+   ** If a client issues the same request twice the result is responsed from an
+   ** internal map holding client requests serial numbers and the results.
+   ** To maintain space by session tracking the paper proposed a LRU semantics for sessions.
+   ** ! This not implemented in this prototype and a session is kept as long as
+   ** the network runs and we assume the client operates without unexpected behavior. **)
+
+  (** The session id, for some client **)
+  Inductive SessionId := session_id (n : nat).
+
+  Definition session_id2nat (si : SessionId) :=
+    match si with
+    | session_id n => n
+    end.
+  Coercion session_id2nat : SessionId >-> nat.
+
+  Definition next_session_id (si : SessionId) : SessionId := session_id (S si).
+
+  Lemma SessionIdDeq : Deq SessionId.
+  Proof.
+    introv. destruct x, y; prove_dec.
+    destruct (deq_nat n n0); prove_dec.
+  Defined.
+
+  (** the initial session id **)
+  Definition session_id0 := session_id 0.
+
+
+  (** A client generates monotcally the ids for its requests. **)
+  Inductive RequestId := request_id (n : nat).
+
+  Definition request_id2nat (ri : RequestId) :=
+    match ri with
+    | request_id n => n
+    end.
+  Coercion request_id2nat : RequestId >-> nat.
+
+  Definition next_request_id (ri : RequestId) : RequestId := request_id (S ri).
+
+  Lemma RequestIdDeq : Deq RequestId.
+  Proof.
+    introv. destruct x, y; prove_dec.
+    destruct (deq_nat n n0); prove_dec.
+  Defined.
+
+  (** the initial request id **)
+  Definition request_id0 := request_id 0.
+
+
+  (** This implementation keps sessions until the network restarts.
+   ** A session is a tuple of some proposed id, the corresponding clien (maybe useless)
+   ** and the last issued request id. The request ids are incremented monotonically. **)
+  Notation Sessions := (list (SessionId * Client * RequestId)).
+
+  (** Return the las found session if some **)
+  Fixpoint get_last_session (s : Sessions) :=
+    match s with
+    | [] => None
+    | x :: [] => Some x
+    | x :: xs => get_last_session xs
+    end.
+
+  Fixpoint last_session_id (s : Sessions) : SessionId :=
+    let session := get_last_session s in
+    match session with
+    | None => session_id0
+    | Some (si, _, _) => si
+    end.
+
+  (** Register some client **)
+  Definition add_session (s : Sessions) (c : Client) : (Sessions * SessionId) :=
+    let si := next_session_id (last_session_id s) in
+    ((si, c, request_id0) :: s, si).
+
+  Fixpoint get_session (s : Sessions) (i : SessionId) :=
+    match s with
+    | [] => None
+    | (si, _, _) @ x :: xs => if (SessionIdDeq si i) then Some x else get_session xs
+    end.
+
+  (** Check if a session is valid. **)
+  Definition valid_session (s : Sessions) (si : SessionId) : bool :=
+    match get_session s si with
+    | None => false
+    | Some _ => true
+    end.
+
+  (** returns wether the request id was already processed or not.
+   ** The implementation returns None, if no session is found,
+   ** false if not processed, true if processed**)
+  Definition already_processed_request (s : Sessions) (si : SessionId) (ri : RequestId) :bool :=
+    match get_session s si with
+    | None => None
+    | Some (_, _, ri') => if RequestIdDeq ri ri' then Some true else Some false
+    end.
+
+  (** If a new request is processed, increment the request id.
+   ** We assume that request ids are incremented monotonically on booth sides. **)
+  Fixpoint increase_request_id (s : Sessions) (si : SessionId) : Sessions :=
+    match s with
+    | [] => s (* do nothing if session not found *)
+    | (si', c, ri) @ x :: xs => if SessionIdDeq si si'
+                              then (si', c, next_request_id ri) :: xs
+                              else x :: increase_request_id xs
+    end.
 
   (*! Terms and progress !*)
   (** Within this protocol the global time is divided into chunks called terms.
-   ** A term starts with the leader election protocol part and
-   **   ends with the supposed failure a leader.
-   ** A term has at most one leader (none if election failed) and
-   **   the current term is maintained by all nodes in the system.
+   ** A term starts with the leader election and ends with the failure a leader.
+   ** A term has at most one leader or none if the election failed.
+   ** The current term is maintained by all nodes in the system.
    ** The main idea is to identify outdated data within the replicated log. **)
   Inductive Term := term (n : nat).
 
-  (** A term is referenced by some number which is increased monotonic. **)
+  (** A term is referenced by some number which is increased monotonically. **)
   Definition term2nat (t : Term) : nat :=
     match t with
     | term n => n
@@ -242,7 +377,7 @@ Section RaftHeader.
   Defined.
 
   (** On boot the first term start with zero. **)
-  Definition initial_term := term 0.
+  Definition term0 := term 0.
 
   (** Test wether term 1 is lesser or equal than term 2. **)
   Definition TermLe (t1 t2 : Term) : bool :=
@@ -256,63 +391,70 @@ Section RaftHeader.
   Definition max_term (t1 t2 : Term) : Term :=
     if TermLe t1 t2 then t2 else t1.
 
-  (*! next index !*)
-  (** The next index is a list of the tuple server id and the
-   ** next possible index for the server.
-   ** The leaders initializes this list every time to last log index + 1.
-   ** The index of a node is increased monotonically if an append entries
-   ** message is send to the node **)
-  Inductive NextIndex :=
-  | next (rep : Rep) (next_index : nat).
+  (*! Index !*)
+  (** The index type is used multiple times as base element for other list types. **)
+  Inductive Index := index (rep : Rep) (index : nat).
 
-  (** A convient notation for a list of next indices **)
-  Notation nindex := (list NextIndex).
-
-
-  (** Create a new next index list out of list of nodes and an initial value **)
-  Fixpoint create_next_index (reps : list Rep) (n : nat) : nindex :=
-    match reps with
-    | [] => []
-    | r :: rs => next r n  :: create_next_index rs n
+  Definition index2nat (i : Index) : nat :=
+    match i with
+    | index _ i => i
     end.
 
-  (** Increase some index **)
-  Definition increase_next_index_e (n : NextIndex) : NextIndex :=
-    match n with
-    | next r ni => next r (ni + 1)
+  Definition index2rep (i : Index) : Rep :=
+    match i with
+    | index r _ => r
+    end.
+
+  Definition next_index (i : Index) : Index :=
+    match i with
+    | index r i => index r (i + 1)
+    end.
+
+  (*! NextIndex !*)
+  (** The next index list is stored on the leader node and maintains a
+   ** list of followers and their next possible log index to use.
+   ** The idea is if outdated log data is found on some follower the leader can decrease
+   ** this index until it finds the first correct log.
+   ** The index for some follower is increased for every unique append entries message. **)
+  Definition NextIndex := list Index.
+
+  (** Create a new next index list. The list is initialized by every new leader
+   ** to its own last log index + 1. **)
+  Fixpoint create_next_index (reps : list Rep) (n : nat) : NextIndex :=
+    match reps with
+    | [] => []
+    | r :: rs => index r n  :: create_next_index rs n
     end.
 
   (** Increase an element in the next index list **)
-  Fixpoint increase_next_index (l : nindex) (rep : Rep) : nindex :=
+  Fixpoint increase_next_index (l : NextIndex) (rep : Rep) : NextIndex :=
     match l with
     | [] => l (* return list if last element reached *)
-    | (next r _) as x :: xs => if (rep_deq r rep)
-                          then increase_next_index_e x :: xs
+    | (index r _) as x :: xs => if (rep_deq r rep)
+                          then next_index x :: xs
                           else x :: increase_next_index xs rep
     end.
 
   (** Return some index if the node is found **)
-  Fixpoint get_next_index (l : nindex) (rep : Rep) : option nat :=
+  Fixpoint get_next_index (l : NextIndex) (rep : Rep) : option nat :=
     match l with
     | [] => None (* the node is not found *)
-    | (next r i) :: xs => if (rep_deq r rep)
+    | (index r i) :: xs => if (rep_deq r rep)
                         then Some i
                         else get_next_index xs rep
     end.
 
-  (*! match index !*)
-  (** The list of match indices is basically the same as the list of next indices
-   ** so the definition are just wrappers about the next index functions.
-   ** The next index stores for a server the index which it knows is replicated by the
-   ** node. One can see this list as mechanism to track the which server has applied
-   ** an append entries message to its local log. **)
-  Notation mindex := (list NextIndex).
+  (*! MatchIndex !*)
+  (** The list of match indices stores for every follower node which log entries
+   ** are already replicated on the follower. If an append entries messages returns
+   ** successfull to the leader it notices the replication by increasing his index.
+   ** TODO: It is unclear what happens if results don't appear in order. **)
+  Definition MatchIndex := list Index.
 
-  Definition create_match_index (reps : list Rep) : mindex := create_next_index reps 0.
-
-  Definition increase_match_index (l : mindex) (rep : Rep) := increase_next_index l rep.
-
-  Definition get_match_index (l : mindex) (rep : Rep) := get_next_index l rep.
+  (** These calls are just wrappers around the next index functions. **)
+  Definition create_match_index (reps : list Rep) : MatchIndex := create_next_index reps 0.
+  Definition increase_match_index (l : MatchIndex) (rep : Rep) := increase_next_index l rep.
+  Definition get_match_index (l : MatchIndex) (rep : Rep) := get_next_index l rep.
 
   (*! Log !*)
   (** An entry in the log takes the term where it is added to the log and
@@ -331,20 +473,20 @@ Section RaftHeader.
     MkEntry
       {
         entry_term : Term;
-        entry : content_type;
+        entry : Content;
       }.
 
   (** Create a new content entry from the type, entry term and content **)
-  Definition new_entry (t : Term) (c : content_type) :=
+  Definition new_entry (t : Term) (c : Content) :=
     MkEntry
       t
       c.
 
   (** Define an abbreviation for the entry list. The comma is enforced by coq. **)
-  Notation "log," := (list Entry) (at level 100).
+  Notation Log := (list Entry).
 
   (** Search for the last entry and return its entry term. **)
-  Fixpoint get_last_log_term (l : log,) : Term :=
+  Fixpoint get_last_log_term (l : Log) : Term :=
     match l with
     | [] => term 0
     | {|entry_term := t|}  :: [] => t
@@ -352,17 +494,17 @@ Section RaftHeader.
     end.
 
   (** Utility function which counts the elements in a log. **)
-  Fixpoint get_last_log_index_util (l : log,) (n : nat) :=
+  Fixpoint get_last_log_index_util (l : Log) (n : nat) :=
     match l with
     | [] => n
     | _ :: xs => get_last_log_index_util xs (n+1)
     end.
 
   (** The first index is 1 **)
-  Definition get_last_log_index (l : log,) : nat := get_last_log_index_util l 1.
+  Definition get_last_log_index (l : Log) : nat := get_last_log_index_util l 1.
 
   (** Check if at position i the entry has the entry term "t". **)
-  Fixpoint check_last_log (i : nat) (t : Term) (l : log,) : bool :=
+  Fixpoint check_last_log (i : nat) (t : Term) (l : Log) : bool :=
     match l with
     | [] => true (* if the log is empty any new entry is accepted *)
     | {|entry_term := t'|} :: [] => if (TermDeq t t') then true else false
@@ -370,7 +512,7 @@ Section RaftHeader.
     end.
 
   (** Take e elements from the log. Start from the end of the list. **)
-  Fixpoint take_from_log_util (e : nat) (l : log,) :=
+  Fixpoint take_from_log_util (e : nat) (l : Log) :=
     match l with
     | [] => ([], 0)
     | x :: xs =>
@@ -378,22 +520,23 @@ Section RaftHeader.
       if (i <? e) then (x :: l, i+1) else (l,i)
     end.
 
-  Definition take_from_log (e : nat) (l : log,) :=
+  Definition take_from_log (e : nat) (l : Log) :=
     let (l, i) := take_from_log_util e l in l.
 
   (** Append new entries to a log  **)
-  Fixpoint append2log (l : log,) (e : list Entry) :=
+  Fixpoint append2log (l : Log) (e : list Entry) :=
     match e with
     | [] => l
     | x :: xs => x :: append2log l xs
     end.
 
+  (** The client issues a new session id by the network.  **)
+  Inductive RegisterClient := register_client (c : Client).
 
-  (*! Request !*)
-  (** A request is issued by some client and contains the client itself for the response message
-   *+ and the command issued to replicate as well as the term number to participate. **)
-  Inductive Request :=
-  | Req (client : Client) (command : content_type) (term : Term).
+  (** To alternate the state a client sends an identifiable message to the network. **)
+  Inductive ClientRequest :=
+  | client_request (client : Client) (session_id : SessionId) (request_id : RequestId)
+                   (command : Content).
 
   (*! Heartbeat and Log replication !*)
   (** The append entries type has two function within the protocol. First it serves as a
@@ -403,8 +546,8 @@ Section RaftHeader.
    ** the last used index number and it's term number. At last the leaders last known
    ** index used and the list of entries to replicate. **)
   Inductive AppendEntries :=
-  | Heartbeat
-  | Replicate (term : Term) (leader : Rep) (last_log_index : nat)
+  | heartbeat
+  | replicate (term : Term) (leader : Rep) (last_log_index : nat)
               (last_log_term : Term) (commit_index : nat) (entry : list Entry).
 
   (*! Election !*)
@@ -412,33 +555,43 @@ Section RaftHeader.
    ** itself, the current term and the index of the last stored log and
    ** it's term number. **)
   Inductive RequestVote :=
-  | Vote (term : Term) (candidate : Rep) (last_log_index : nat) (last_log_term : Term).
+  | request_vote (term : Term) (candidate : Rep) (last_log_index : nat) (last_log_term : Term).
 
   (*! Results !*)
   (** The result type provides the different results used within the protocol. **)
   Inductive Result :=
   (** The leader sends the client the response if his state machine. **)
-  | ClientRes (result : nat)
+  | client_res (result : nat)
   (** The follower responses to the leader if the issued requests succeds and
    ** the current term to update the leader. **)
-  | AppendEntriesRes (success : bool) (term : Term)
+  | append_entries_res (success : bool) (term : Term)
   (** A node response to a request vote wether it votes the calling candidate
    ** and it's current term to updat the requesting node. **)
-  | RequestVoteRes (vote_granted : bool) (term : Term).
+  | request_vote_res (vote_granted : bool) (term : Term)
+  (** Return if the client is registered and its new session id **)
+  | register_client_res (status: bool) (session_id : SessionId) (leader : option Rep).
 
   (*! Messages !*)
   (** Define the messages which can be used within the system for communication
    ** between the nodes. A message takes one inductive type due to the state machine definition.
    ** Authentication is currently not provided. **)
-  Inductive Raftmsg :=
+  Inductive RaftMsg :=
+  (* Before communicating with the network a client registers itself at the network. *)
+  | register_msg (register : RegisterClient)
+  (* Respond to a register message. *)
+  | register_result_msg (result : Result)
+  (* If the sessions changes and a new client enters the network
+   * the leader broadcast the new sessions to all followers.
+   * This is done to find duplicated request early and new leaders didn't forget clients. *)
+  | broadcast_sessions_msg (sessions : Sessions)
   (* A client request is the command issued by the client to modify the overall state.
    * As a parameter the client sends its own id, some sequence number to eliminate duplacte
    * requests and the command to execute. *)
-  | RequestMsg (request : Request)
+  | request_msg (request : ClientRequest)
   (* The response is sent by the leader after it applies the issued command to it's
    * own state machine and the first round of AppendEntries send through the network.
    * The result is taken from the result of the leader state machine. *)
-  | ResponseMsg (result : Result)
+  | response_msg (result : Result)
   (* The append entries messages is invoked by the leader to replicate some client
    * request by all followers within the system.
    * If followers crash, run slowly or if network packets are dropped the leader tries
@@ -446,37 +599,40 @@ Section RaftHeader.
    *
    * The message has a second function as heartbeat when issued without log entries
    * to be replicated by the followers. No result are expected from heartbeat messages. *)
-  | AppendEntriesMsg (entries : AppendEntries)
+  | append_entries_msg (entries : AppendEntries)
   (* If the leader issued some log replication the follower response wether the
    * request succeds and it's current term number to inform the leader what problem
    * happens. *)
-  | AppendEntriesResultMsg (result : Result)
+  | append_entries_result_msg (result : Result)
   (* A follower issues a request vote message if it thinks the leader is faulty.
    * It transitions to candidate state and starts the leader election. *)
-  | RequestVoteMsg (vote : RequestVote)
+  | request_vote_msg (vote : RequestVote)
   (* The response vote messages is returned by processing some request vote message.
    * It indicates to the requesting client wether it recieves a vote from this
    * node or not. *)
-  | ResponseVoteMsg (result : Result)
+  | response_vote_msg (result : Result)
   (* The forwarding is used if some client send a request to a none leader replica.
    * It encapsulates the message and sends it to the current leader. *)
-  | ForwardMsg (msg : Raftmsg).
+  | forward_msg (msg : RaftMsg).
 
   (** Bind the implemented messages to the abstract velisarios type class. **)
-  Global Instance Raft_I_Msg : Msg := MkMsg Raftmsg.
+  Global Instance Raft_I_Msg : Msg := MkMsg RaftMsg.
 
   (** Forall messages some state shall be defined wether this messages comes
    ** from outside the network (client request) or is used within the network
    ** (protocol request) or within the node (internal message). **)
-  Definition Raftmsg2status (m : Raftmsg) : msg_status :=
+  Definition Raftmsg2status (m : RaftMsg) : msg_status :=
     match m with
-    | RequestMsg _             => MSG_STATUS_EXTERNAL
-    | ResponseMsg _            => MSG_STATUS_PROTOCOL
-    | AppendEntriesMsg _       => MSG_STATUS_PROTOCOL
-    | AppendEntriesResultMsg _ => MSG_STATUS_PROTOCOL
-    | RequestVoteMsg _         => MSG_STATUS_PROTOCOL
-    | ResponseVoteMsg _        => MSG_STATUS_PROTOCOL
-    | ForwardMsg _             => MSG_STATUS_PROTOCOL
+    | register_msg _              => MSG_STATUS_EXTERNAL
+    | register_result_msg _       => MSG_STATUS_PROTOCOL
+    | broadcast_sessions_msg _    => MSG_STATUS_PROTOCOL
+    | request_msg _               => MSG_STATUS_EXTERNAL
+    | response_msg _              => MSG_STATUS_PROTOCOL
+    | append_entries_msg _        => MSG_STATUS_PROTOCOL
+    | append_entries_result_msg _ => MSG_STATUS_PROTOCOL
+    | request_vote_msg _          => MSG_STATUS_PROTOCOL
+    | response_vote_msg _         => MSG_STATUS_PROTOCOL
+    | forward_msg _               => MSG_STATUS_PROTOCOL
     end.
 
   (** Bind the real message states to the abstract definition. **)
