raft/protocols/Raft/Raft.v
@@ -22,56 +22,64 @@ Section Raft.
   Context { raft_context : RaftContext }.
 
   (** redeclare the notations **)
-  Notation Nindex := (list NextIndex).
-  Notation Mindex := (list NextIndex).
   Notation Log := (list Entry).
-  Notation Commit_log := (list Entry).
+  Notation Sessions := (list (SessionId * Client)).
+
+  (* Notation Nindex := (list NextIndex). *)
+  (* Notation Mindex := (list NextIndex). *)
+  (* Notation Commit_log := (list Entry). *)
 
   (*! Leader state !*)
   (** The leader state indicates the node as leader and is reinitialized after every
    ** election round. **)
 
-  Record RaftLeaderState :=
+  Record LeaderState :=
     Build_Leader_State
       {
-        (* Indicates wether the node is the leader. *)
-        is_leader : bool;
         (* Volatile; reset after election -
          * The list of followers and the next possible index to send to the follower.
          * Try list index as node marker -> (node_num, next_index)*)
-        next_index : Nindex;
+        next_index : NextIndex;
         (* Volatile; reset after election -
          * The list of servers and their index of the highest log entry.
          * Try the list index as a marker for the node id. *)
-        match_index : Mindex;
+        match_index : MatchIndex;
       }.
 
   (** This definition is used to initialize the network, because
    ** their is no leader in the beginning. **)
-  Definition no_leader_state : RaftLeaderState :=
-    Build_Leader_State false [] [].
+  Definition no_leader_state : LeaderState :=
+    Build_Leader_State [] [].
 
   (** This definition is used only for testing. It creates an initial leader *)
   (*  ** with a provided follower network. **)
-  Definition init_leader_state (followers : list nat) : RaftLeaderState :=
+  Definition init_leader_state (followers : list nat) : LeaderState :=
     let reps := List.map nat2rep followers in
-    Build_Leader_State true
-                       (create_next_index reps 0)
+    Build_Leader_State (create_next_index reps 0)
                        (create_match_index reps).
 
   (** This definition reinitializes the node that has won the leader election. **)
-  Definition after_election_leader (next_index : nat) (followers : list Rep) : RaftLeaderState :=
-    Build_Leader_State true
-                       (create_next_index followers next_index)
+  Definition after_election_leader (next_index : nat) (followers : list Rep) : LeaderState :=
+    Build_Leader_State (create_next_index followers next_index)
                        (create_match_index followers).
 
+ 
+
   (*! Node State !*)
+  (** Model the different states a server can be which are leader, follower or candidate. **)
+  Inductive NodeState :=
+  | leader (l : LeaderState)
+  | follower
+  | candidate.
+
   (** The state describes the parts that are persistent on all nodes. **)
   Record RaftState :=
     Build_State
       {
         (* The last term the node has seen, this should be persitent over crashes. *)
         current_term : Term;
+        (* maintain the client sessions *)
+        sessions: Sessions;
         (* The candidate this node voted for the current term or null if none *)
         voted_for : (option nat);
         (* The replicated log data which should be persitent over crashes
@@ -81,10 +89,6 @@ Section Raft.
          * The index provides information to which request the global state machine
          * has applied the requests. *)
         commit_index : nat;
-        (* Since we don't implement a real state machine where the commited logs
-         * gets applied (out of scope) a second list is used as dummy to show the mechanics.
-         * If a majority agrees on a log entry the entry gets copied to the commited_log. *)
-        committed : Commit_log;
         (* Volatile - The last log index applied to the state machine. *)
         last_applied : nat;
         (* the timeout in secs after which a new election is triggered.
@@ -92,9 +96,9 @@ Section Raft.
          * with some offset like node * 10 + timeout *)
         node_timeout : nat;
         (* the node local state machine *)
-        sm_state : RaftSM_state;
+        sm_state : RaftSM;
         (* The leader state if the node is the leader *)
-        leader : RaftLeaderState;
+        node_state : NodeState;
         (* The term leader *)
         current_leader : (option Rep);
         (* the list of other servers excluding this one *)
@@ -102,119 +106,112 @@ Section Raft.
       }.
 
   (** The initial state for all nodes. **)
-  Definition initial_state : RaftState :=
+  Definition state0 : RaftState :=
     Build_State
-      initial_term (* zero at first boot *)
+      term0 (* zero at first boot *)
+      [] (* No clients added *)
       None (* voted for no one. *)
       [] (* no log entries stored *)
       0 (* no commit done *)
-      [] (* empty commited log *)
       0 (* nothing applied to state machine *)
       5 (* some way of defining an offset is needed *)
       RaftSM_initial_state (* defined within the raft context *)
-      no_leader_state (* at default no one is leader *)
-      None (* set leader to none *)
+      follower (* at default no one is leader *)
+      None (* no leader known *)
       [].
-
-  (** An initial state for replicas with the leader set to replica 0. **)
-  Definition initial_faked_leader_state : RaftState :=
-    Build_State
-      initial_term (* zero at first boot *)
-      None (* voted for no one. *)
-      [] (* no log entries stored *)
-      0 (* no commit done *)
-      [] (* empty commited log *)
-      0 (* nothing applied to state machine *)
-      5 (* some way of defining an offset is needed *)
-      RaftSM_initial_state (* defined within the raft context *)
-      no_leader_state (* at default no one is leader *)
-      (Some (nat2rep 0)) (* set leader to 0 *)
-      [] (* empty list of nodes *).
-
-
-  (** An initial leader state which should only used for testing. **)
-  Definition initial_leader_state : RaftState :=
-    Build_State
-      initial_term (* zero at first boot *)
-      None (* voted for no one. *)
-      [] (* no log entries stored *)
-      0 (* no commit done *)
-      [] (* empty commited log *)
-      0 (* nothing applied to state machine *)
-      5 (* some way of defining an offset is needed *)
-      RaftSM_initial_state (* defined within the raft context *)
-      (init_leader_state [1, 2, 3]) (* define as leader with 3 followers *)
-      (Some (nat2rep 0)) (* set leader to 0 for testing *)
-      [1, 2, 3] (* empty list of nodes *).
 
   (*! State transitions !*)
   (** If some leader is byzantine a new election starts and the term number is increased **)
   Definition increment_term_num (s : RaftState) : RaftState :=
     Build_State
       (next_term (current_term s))
+      (sessions s)
       (voted_for s)
       (log s)
       (commit_index s)
-      (committed s)
       (last_applied s)
       (node_timeout s)
       (sm_state s)
-      (leader s)
+      (node_state s)
       (current_leader s)
       (nodes s).
 
   (** replace the nodes log **)
-  Definition update_log (s : RaftState) (l : list Entry) : RaftState :=
+  Definition update_log (s : RaftState) (l : Log) : RaftState :=
     Build_State
       (current_term s)
+      (sessions s)
       (voted_for s)
       l
       (commit_index s)
-      (committed s)
       (last_applied s)
       (node_timeout s)
       (sm_state s)
-      (leader s)
+      (node_state s)
       (current_leader s)
       (nodes s).
 
-    (** replace the commit index **)
-  Definition update_commit_log (s : RaftState) (ci : nat) (l : Commit_log) : RaftState :=
+    (** Update the state machine **)
+  Definition update_sm (s : RaftState) (ci : nat) (sm : RaftSM) : RaftState :=
     Build_State
       (current_term s)
+      (sessions s)
       (voted_for s)
       (log s)
       ci
-      l
       (last_applied s)
       (node_timeout s)
-      (sm_state s)
-      (leader s)
+      sm
+      (node_state s)
       (current_leader s)
       (nodes s).
 
-  Definition update_leader (s : RaftState) (l : Rep) : RaftState :=
+  Definition update_node_type (s : RaftState) (l : Rep) : RaftState :=
     Build_State
       (current_term s)
+      (sessions s)
       (voted_for s)
       (log s)
       (commit_index s)
-      (committed s)
       (last_applied s)
       (node_timeout s)
       (sm_state s)
-      (leader s)
+      (node_state s)
       (Some l)
+      (nodes s).
+
+  Definition update_sessions (s : RaftState) (se : Sessions) : RaftState :=
+    Build_State
+      (current_term s)
+      se
+      (voted_for s)
+      (log s)
+      (commit_index s)
+      (last_applied s)
+      (node_timeout s)
+      (sm_state s)
+      (node_state s)
+      (current_leader s)
       (nodes s).
 
 
   (*! Utilities !*)
-
   (** TODO: This seems like vodoo, at the moment, where does reps come from. **)
   Definition other_replicas (r : Rep) : list Rep := remove_elt rep_deq r reps.
-  Definition other_names (r : Rep) : list name := map Raftreplica (other_replicas r).
+  Definition other_names (r : Rep) : list name := map replica (other_replicas r).
 
-  Definition leading (s : RaftState) : bool := (is_leader (leader s)).
+  (** Check if a node is the leader **)
+  Definition is_leader (s : RaftState) : bool :=
+    match (node_state s) with
+    | leader _ => true
+    | _ => false
+    end.
+
+  Definition get_leader (s : RaftState) : option LeaderState :=
+    match (node_state s) with
+    | leader l => (Some l)
+    | _ => None
+    end.
 
   (*! The message handling - Update function !*)
   (** Each possible transition has it's own handle function for the input message.
@@ -229,28 +226,28 @@ Section Raft.
    ** 2. If this node has no leader (newly started network) it currently drops the request.
    ** 3. The reciever forwards the message if it is not the leader
    ** 4. Otherwise, it unpacks all messages and sends the innerst message to itself **)
-  Definition create_forward_msg (s : option Rep) (o : Raftmsg) : DirectedMsgs :=
+  Definition create_forward_msg (s : option Rep) (o : RaftMsg) : DirectedMsgs :=
     match s with
       (* we have no new current leader, maybe the system was recently initialized and
        * no leader is elected yet. TODO: Ignore the message at the moment *)
     | None => []
-    | Some l => [MkDMsg (ForwardMsg o) [Raftreplica l] 0]
+    | Some l => [MkDMsg (forward_msg o) [replica l] 0]
     end.
 
   (** Unwrap all possible wrapped forwarded messages and return the original message. **)
-  Fixpoint unpack_forwards (f : Raftmsg) : Raftmsg :=
+  Fixpoint unpack_forwards (f : RaftMsg) : RaftMsg :=
     match f with
-    | ForwardMsg f => unpack_forwards f
+    | forward_msg f => unpack_forwards f
     | f => f
     end.
 
   (** L - Handle fowarded message - unpack and send original message to self. **)
-  Definition Rafthandle_forward_msg (slf : Rep) : Update RaftState Raftmsg DirectedMsgs :=
+  Definition handle_forward_msg (slf : Rep) : Update RaftState RaftMsg DirectedMsgs :=
     fun state f =>
-      if leading state then
+      if is_leader state then
         (* maybe there is a better way of handling this. *)
         let msg := unpack_forwards f in
-        (Some state, [MkDMsg msg [(Raftreplica slf)] 0])
+        (Some state, [MkDMsg msg [(replica slf)] 0])
       (* Either forward the message to the current leader or ignore it.
        * Maybe a TODO to handle the first encountered messages if there is no leader. *)
       else (Some state, (create_forward_msg (current_leader state) f)).
@@ -266,16 +263,20 @@ Section Raft.
    ** 5. The follower repsonds to the leader with it's result and the current term
    ** 6. If the leader gets a majority of successfull repsonses from the followers
    **    it commits the log entry to the commited_log. **)
+  (* TODO: resend append entry calls indefinitely if followers does not answer
+   * TODO: apply log entry as committed if majority of followers succeds
+   * TODO: leader send response to server
+   * TODO: deal with log inconsistency -> the leader needs to detect the last valid log. *)
 
   (** Create the replication messages which are send to the followers
    ** To make this easy the request sends a nat as cmd to the leader and
    ** the leader converts this into a single entry list for the log replication. **)
   Definition create_append_msg (slf : Rep) (s : RaftState) (entries: list Entry) : DirectedMsgs :=
-    let leader := leader s in
+    let leader := (get_leader s) in
     let llt := get_last_log_term (log s) in
     let lli := get_last_log_index (log s) in
-    let msg := Replicate (current_term s) slf lli llt (commit_index s) entries in
-    [MkDMsg (AppendEntriesMsg msg) (other_names slf) 0].
+    let msg := replicate (current_term s) slf lli llt (commit_index s) entries in
+    [MkDMsg (append_entries_msg msg) (other_names slf) 0].
 
   (** 1. If the next used log index is equal to the internal log index
    ** 1.1 check if the terms of the entries are matching and
@@ -308,18 +309,19 @@ Section Raft.
   Definition commit (s : RaftState) (ci : nat) :=
     let new_ci := new_commit_index s ci in
     let log := take_from_log new_ci (log s) in
-    (update_commit_log s new_ci log).
+    (update_sm s new_ci (sm_state s)).
 
   (** L - Handle client input to the system. **)
   (** Forward the message if the request reaches the wrong node.
    ** As leader generate the entries from the request and apply the entries to the
    ** internal log. Afterwards send AppendEntries messages to the followers. **)
-  Definition Rafthandle_request (slf : Rep) : Update RaftState Request DirectedMsgs :=
+  Definition handle_request (slf : Rep) : Update RaftState ClientRequest DirectedMsgs :=
     fun state r =>
-      if leading state then
+      if is_leader state then
         (* We are the leader *)
         match r with
-        | Req client cmd t =>
+        | client_request c si ri cmd =>
+          if valid_session (sessions state) si then
           let entry := [new_entry (term (current_term state)) cmd] in
           (* create the replication messages for all leaders *)
           let dmsgs := create_append_msg slf state entry in
@@ -328,10 +330,12 @@ Section Raft.
           let lli := get_last_log_index (log state) in
           let new_state := (update_log state (append_entries2log entry lli (current_term state) state)) in
           (Some new_state, dmsgs)
+          else
+            (Some state, []) (* ignore the message if there is no session *)
         end
       else
       (* Some node that forwards *)
-        let msg := create_forward_msg (current_leader state) (RequestMsg r) in
+        let msg := create_forward_msg (current_leader state) (request_msg r) in
         (Some state, msg).
 
   (** F - Handle append entries messages which are used as heartbeat and log replication. **)
@@ -342,38 +346,38 @@ Section Raft.
    ** 3. Check if the entries could be applied to the internal log
    ** 3.1 Ignore the request if the current term doesn't match or the entry is already there (index + term)
    ** 3.2 Apply the entries to the internal log by removing false entries and response with success and the current term **)
-  Definition Rafthandle_append_entries (slf : Rep) : Update RaftState AppendEntries DirectedMsgs :=
+  Definition handle_append_entries (slf : Rep) : Update RaftState AppendEntries DirectedMsgs :=
     fun state msg =>
-      if leading state then (Some state, []) (* this shouldn't happen *)
+      if is_leader state then (Some state, []) (* this shouldn't happen *)
       else
         match msg with
         (* leader timeout reset *)
-        | Heartbeat => (Some state, []) (* TODO: ignore election at the moment *)
+        | heartbeat => (Some state, []) (* TODO: ignore election at the moment *)
         (* log replication *)
-        | Replicate t l lli llt ci entries =>
+        | replicate t l lli llt ci entries =>
           if (TermLt t (current_term state)) then
             (* reply false if the replication term is lower than the current term *)
-            let result := AppendEntriesRes false (current_term state) in
-            (Some state, [MkDMsg (AppendEntriesResultMsg result) [Raftreplica l] 10])
+            let result := append_entries_res false (current_term state) in
+            (Some state, [MkDMsg (append_entries_result_msg result) [replica l] 10])
           else
             if (negb (check_last_log lli llt (log state))) then
               (* reply false if the last log index or term does not match *)
-              let result := AppendEntriesRes false (current_term state) in
-              (Some state, [MkDMsg (AppendEntriesResultMsg result) [Raftreplica l] 20])
+              let result := append_entries_res false (current_term state) in
+              (Some state, [MkDMsg (append_entries_result_msg result) [replica l] 20])
             else
               (* handle the replication request *)
               let new_log := append_entries2log entries lli t state in
-              let result := AppendEntriesRes true (current_term state) in
+              let result := append_entries_res true (current_term state) in
               let s := (update_log state new_log) in
               let s' := (commit s ci) in
-              let s'' := (update_leader s' l) in
-              (Some s'', [MkDMsg (AppendEntriesResultMsg result) [Raftreplica l] 0])
+              let s'' := (update_node_type s' l) in
+              (Some s'', [MkDMsg (append_entries_result_msg result) [replica l] 0])
         end.
 
   (** L - Handle results messages from followers. **)
-  Definition Rafthandle_append_entries_result (slf : Rep) : Update RaftState Result DirectedMsgs :=
+  Definition handle_append_entries_result (slf : Rep) : Update RaftState Result DirectedMsgs :=
     fun state r =>
-      if leading state then
+      if is_leader state then
         (* let c := [Raftclient client] in *)
         (* (Some state, [MkDMsg (ResponseMsg (ClientRes cmd)) c 0]) *)
         (Some state, [])
@@ -381,56 +385,133 @@ Section Raft.
       else (Some state, []). (* this shoudln't happen *)
 
   (** C - Handle incoming votes from candidates. **)
-  Definition Rafthandle_request_vote (slf : Rep) : Update RaftState RequestVote DirectedMsgs :=
+  Definition handle_request_vote (slf : Rep) : Update RaftState RequestVote DirectedMsgs :=
     fun state _ => (Some state, []).
 
   (** C - Handle incoming voting results from candidates. **)
-  Definition Rafthandle_response_vote (slf : Rep) : Update RaftState Result DirectedMsgs :=
+  Definition handle_response_vote (slf : Rep) : Update RaftState Result DirectedMsgs :=
     fun state _ => (Some state, []).
 
-  (** Cl - The client handles the response from a node - currently nothing **)
-  Definition Rafthandle_response (slf : Rep) : Update RaftState Result DirectedMsgs :=
+  (*! Register some client at the network !*)
+  Definition create_register_result_msg (c : Client) (r : Result) :=
+    [MkDMsg (register_result_msg r) [client c] 0].
+ 
+  Definition create_broadcast_msg (slf : Rep) (b : RaftMsg) :=
+    [MkDMsg b (other_names slf) 0].
+
+  (** L _ Handle incoming new clients **)
+  (** Some client sends an empty register_client message and the leader creates a session
+   ** for this client. This session is distributed across the network.
+   **
+   ** The papers approach is to handle regiter messages like normal log replication messages.
+   ** No checks are done if the distribution was successfully since all client messages
+   ** are forwarded to the leader. So, the disribution is implemented as a showcase. **)
+  Definition handle_register (slf : Rep) : Update RaftState RegisterClient DirectedMsgs :=
+    fun state msg =>
+      if is_leader state then
+        match msg with (* we're the leader and register the client *)
+        | register_client c =>
+          let (sessions, id) := add_session (sessions state) c in
+          let s' := update_sessions state sessions in
+          let result := register_client_res true id (Some slf) in
+          let broadcast := create_broadcast_msg slf (broadcast_sessions_msg sessions) in
+          (Some s', create_register_result_msg c result ++ broadcast)
+        end
+      else
+        let forward := create_forward_msg (current_leader state) (register_msg msg) in
+        (Some state, forward). (* forward messsage if we're not the leader *)
+
+  (** F - Handle a leader brodacast with new sessions by just replacing the own sessions. **)
+  Definition handle_sessions_broadcast (slf : Rep) : Update RaftState Sessions DirectedMsgs :=
+    fun state sessions =>
+      if is_leader state then (Some state, [])
+      else (Some (update_sessions state sessions), []).
+
+  (*! maybe useless !*)
+  (** Cl - A client handles the response for the register message of the client - nothing atm **)
+  Definition handle_register_result (slf : Rep) : Update RaftState Result DirectedMsgs :=
+    fun state _ => (Some state, []).
+
+  (** Cl -  The client handles the response from a node - currently nothing **)
+  Definition handle_response (slf : Rep) : Update RaftState Result DirectedMsgs :=
     fun state _ => (Some state, []).
 
 
   (** The main update function which calls the appropriate handler function
    ** for the incoming message type. **)
-  Definition Raftreplica_update (slf : Rep) : MUpdate RaftState :=
+  Definition replica_update (slf : Rep) : MUpdate RaftState :=
     fun state m =>
       match m with
-      | RequestMsg d => Rafthandle_request slf state d
-      | ResponseMsg d => Rafthandle_response slf state d
-      | AppendEntriesMsg d => Rafthandle_append_entries slf state d
-      | AppendEntriesResultMsg d => Rafthandle_append_entries_result slf state d
-      | RequestVoteMsg d => Rafthandle_request_vote slf state d
-      | ResponseVoteMsg d => Rafthandle_response_vote slf state d
-      | ForwardMsg msg => Rafthandle_forward_msg slf state msg
+      | register_msg d => handle_register slf state d
+      | register_result_msg d => handle_register_result slf state d
+      | broadcast_sessions_msg d => handle_sessions_broadcast slf state d
+      | request_msg d => handle_request slf state d
+      | response_msg d => handle_response slf state d
+      | append_entries_msg d => handle_append_entries slf state d
+      | append_entries_result_msg d => handle_append_entries_result slf state d
+      | request_vote_msg d => handle_request_vote slf state d
+      | response_vote_msg d => handle_response_vote slf state d
+      | forward_msg msg => handle_forward_msg slf state msg
       end.
 
+
+  (*! Define fake states for testing !*)
+ Definition initial_faked_leader_state : RaftState :=
+    Build_State
+      term0 (* zero at first boot *)
+      [] (* *)
+      None (* voted for no one. *)
+      [] (* no log entries stored *)
+      0 (* no commit done *)
+      0 (* nothing applied to state machine *)
+      5 (* some way of defining an offset is needed *)
+      RaftSM_initial_state (* defined within the raft context *)
+      follower (* at default no one is leader *)
+      (Some (nat2rep 0)) (* set leader to 0 *)
+      [] (* empty list of nodes *).
+
+
+  (** An initial leader state which should only used for testing. **)
+  Definition initial_leader_state : RaftState :=
+    Build_State
+      term0 (* zero at first boot *)
+      []
+      None (* voted for no one. *)
+      [] (* no log entries stored *)
+      0 (* no commit done *)
+      0 (* nothing applied to state machine *)
+      5 (* some way of defining an offset is needed *)
+      RaftSM_initial_state (* defined within the raft context *)
+      (leader (init_leader_state [1, 2, 3])) (* define as leader with 3 followers *)
+      (Some (nat2rep 0)) (* set leader to 0 for testing *)
+      [1, 2, 3] (* set follower nodes *).
+
+
   (*! System definitions !*)
+  (* match node names with state machines *)
+  Definition Raftnstate (n : name) :=
+    match n with
+    | replica _ => RaftState
+    | _ => unit
+    end.
+
   (** Define the actual state machine used by velisarios **)
-  Definition RaftreplicaSM (slf : Rep) : MStateMachine _ (* let the compiler guess ? *) :=
+  Definition RaftReplicaSM (slf : Rep) : MStateMachine _ (* let the compiler guess ? *) :=
     mkSM
-      (Raftreplica_update slf)
-      (initial_faked_leader_state).
+      (replica_update slf)
+      (state0).
 
   (** This binding should only used for testing. **)
   Definition RaftLeaderreplicaSM (slf : Rep) : MStateMachine _ (* let the compiler guess ? *) :=
     mkSM
-      (Raftreplica_update slf)
+      (replica_update slf)
       (initial_leader_state).
 
-  (* match node names with state machines *)
-  Definition Raftnstate (n : name) :=
-    match n with
-    | Raftreplica _ => RaftState
-    | _ => unit
-    end.
 
   Definition Raftsys : MUSystem Raftnstate :=
     fun name =>
       match name return StateMachine (Raftnstate name) msg DirectedMsgs with
-      | Raftreplica n => RaftreplicaSM n
+      | replica n => RaftReplicaSM n
       | _ => MhaltedSM tt
       end.
 
